@@ -499,3 +499,5 @@ import Xv6.ProofBeginOp
 import Xv6.LinkBeginOp
 import Xv6.ProofSysSync
 import Xv6.LinkSysSync
+import Xv6.ProofLogWrite
+import Xv6.LinkLogWrite
